Merge 'preform and 'form

Abstract_Formula.thy
@@ -5,87 +5,113 @@ imports
   "~~/src/HOL/Library/Stream"
   Indexed_FSet
 begin
-
-type_synonym 'a annotated = "('a \<times> nat)"
-
 locale Abstract_Formulas =
-  fixes freshen :: "nat \<Rightarrow> 'preform \<Rightarrow> 'form"
-  fixes pre_fv :: "'preform \<Rightarrow> 'var set"
-  fixes fv :: "'form \<Rightarrow> 'var annotated set"
+  fixes freshenV :: "nat \<Rightarrow> 'var \<Rightarrow> 'var"
+  fixes rename :: "('var \<Rightarrow> 'var) \<Rightarrow> ('form \<Rightarrow> 'form)"
+  fixes fv :: "'form \<Rightarrow> 'var set"
   fixes subst :: "'subst \<Rightarrow> 'form \<Rightarrow> 'form"
-  fixes ran_fv :: "'subst \<Rightarrow> 'var annotated set"
-  fixes closed :: "'preform \<Rightarrow> bool"
-  fixes anyP :: "'preform"
-  assumes fv_freshen': "fv (freshen a pf) = (\<lambda> v. (v,a)) ` pre_fv pf"
-  assumes subst_no_vars: "pre_fv pf = {} \<Longrightarrow> fv (subst s f) = {}"
+  fixes ran_fv :: "'subst \<Rightarrow> 'var set"
+  fixes anyP :: "'form"
+  assumes freshenV_eq_iff[simp]: "freshenV a v = freshenV a' v' \<longleftrightarrow> a = a' \<and> v = v'"
+  assumes fv_rename: "fv (rename p f) = p ` fv f"
+  assumes rename_closed: "fv f = {} \<Longrightarrow> rename p f = f"
+  assumes subst_closed: "fv f = {} \<Longrightarrow> subst s f = f"
   assumes fv_subst: "fv (subst s f) \<subseteq> fv f \<union> ran_fv s"
-  assumes closed_pre_fv: "closed pf \<Longrightarrow> pre_fv pf = {}"
-  assumes closed_eq: "closed pf1 \<Longrightarrow> subst s1 (freshen a1 pf1) = subst s2 (freshen a2 pf2) \<longleftrightarrow> pf1 = pf2"
-  assumes anyP_is_any: "\<exists> s. subst s (freshen a anyP) = f"
+  assumes anyP_is_any': "\<exists> s. subst s (rename (freshenV a) anyP) = f"
 begin
-  definition freshenV :: "nat \<Rightarrow> 'var \<Rightarrow>  'var annotated" where "freshenV a v = (v,a)"
-  lemma fv_freshen: "fv (freshen a pf) = freshenV a ` pre_fv pf"
-    using freshenV_def fv_freshen' by auto
-  lemma freshenV_eq_iff[simp]: "freshenV a v = freshenV a' v' \<longleftrightarrow> a = a' \<and> v = v'"
-    by (auto simp add: freshenV_def)
+  definition freshen :: "nat \<Rightarrow> 'form \<Rightarrow> 'form" where
+    "freshen n = rename (freshenV n)"
+
+  lemma fv_freshen: "fv (freshen a f) = freshenV a ` fv f"
+    unfolding freshen_def by (rule fv_rename)
+
+  lemma anyP_is_any: "\<exists> s. subst s (freshen a anyP) = f"
+    unfolding freshen_def by (rule anyP_is_any')
+
+  definition closed :: "'form \<Rightarrow> bool" where "closed f \<longleftrightarrow> fv f = {}"
+  lemma closed_fv: "closed f \<Longrightarrow> fv f = {}" unfolding closed_def by auto
+
+  lemma closed_eq:
+    assumes "closed f1"
+    assumes "closed f2"
+    shows "subst s1 (freshen a1 f1) = subst s2 (freshen a2 f2) \<longleftrightarrow> f1 = f2"
+  using assms
+    by (auto simp add: closed_def freshen_def fv_freshen subst_closed rename_closed)
+
   lemma freshenV_range_eq_iff[simp]: "freshenV a v \<in> range (freshenV a') \<longleftrightarrow> a = a'"
     by auto
 end
 
-datatype ('preform, 'var) antecedent =
-  Antecedent (a_hyps: "'preform fset") (a_conc: "'preform") (a_fresh: "'var set")
+datatype ('form, 'var) antecedent =
+  Antecedent (a_hyps: "'form fset") (a_conc: "'form") (a_fresh: "'var set")
 
-abbreviation plain_ant :: "'preform \<Rightarrow> ('preform, 'var) antecedent"
+abbreviation plain_ant :: "'form \<Rightarrow> ('form, 'var) antecedent"
   where "plain_ant f \<equiv> Antecedent {||} f {}"
 
 locale Abstract_Rules =
-  Abstract_Formulas freshen pre_fv fv subst ran_fv closed anyP
-  for freshen :: "nat \<Rightarrow> 'preform \<Rightarrow> 'form"
-  and pre_fv :: "'preform \<Rightarrow> 'var set"
-  and fv :: "'form \<Rightarrow> 'var annotated set"
+  Abstract_Formulas freshenV rename fv subst ran_fv anyP
+  for freshenV :: "nat \<Rightarrow> 'var \<Rightarrow> 'var"
+  and rename  :: "('var \<Rightarrow> 'var) \<Rightarrow> ('form \<Rightarrow> 'form)"
+  and fv :: "'form \<Rightarrow> 'var set"
   and subst :: "'subst \<Rightarrow> 'form \<Rightarrow> 'form" 
-  and ran_fv :: "'subst \<Rightarrow> ('var \<times> nat) set" 
-  and closed :: "'preform \<Rightarrow> bool" 
-  and anyP :: "'preform" +
-  fixes antecedent :: "'rule \<Rightarrow> ('preform, 'var) antecedent list"
-  fixes consequent :: "'rule \<Rightarrow> 'preform list"
+  and ran_fv :: "'subst \<Rightarrow> 'var set" 
+  and anyP :: "'form" +
+  fixes antecedent :: "'rule \<Rightarrow> ('form, 'var) antecedent list"
+  fixes consequent :: "'rule \<Rightarrow> 'form list"
   and rules :: "'rule stream"
 begin
-  definition f_antecedent :: "'rule \<Rightarrow> ('preform, 'var) antecedent fset"
+  definition f_antecedent :: "'rule \<Rightarrow> ('form, 'var) antecedent fset"
     where "f_antecedent r = fset_from_list (antecedent r)"
   definition "f_consequent r = fset_from_list (consequent r)"
 end
 
 locale Abstract_Task =
-  Abstract_Rules freshen pre_fv fv subst ran_fv closed anyP  antecedent consequent rules
-  for freshen :: "nat \<Rightarrow> 'preform \<Rightarrow> 'form" 
-    and pre_fv :: "'preform \<Rightarrow> 'var set" 
-    and fv :: "'form \<Rightarrow> 'var annotated set" 
+  Abstract_Rules freshenV rename fv subst ran_fv anyP  antecedent consequent rules
+  for freshenV :: "nat \<Rightarrow> 'var \<Rightarrow> 'var"
+    and rename  :: "('var \<Rightarrow> 'var) \<Rightarrow> ('form \<Rightarrow> 'form)"
+    and fv :: "'form \<Rightarrow> 'var set"
     and subst :: "'subst \<Rightarrow> 'form \<Rightarrow> 'form" 
-    and ran_fv :: "'subst \<Rightarrow> 'var annotated set" 
-    and closed :: "'preform \<Rightarrow> bool" 
-    and anyP :: "'preform" 
-    and antecedent :: "'rule \<Rightarrow> ('preform, 'var) antecedent list"
-    and consequent :: "'rule \<Rightarrow> 'preform list" 
+    and ran_fv :: "'subst \<Rightarrow> 'var set" 
+    and anyP :: "'form"
+    and antecedent :: "'rule \<Rightarrow> ('form, 'var) antecedent list"
+    and consequent :: "'rule \<Rightarrow> 'form list" 
     and rules :: "'rule stream" +
-  fixes assumptions :: "'preform list"
-  fixes conclusions :: "'preform list"
+  fixes assumptions :: "'form list"
+  fixes conclusions :: "'form list"
   assumes assumptions_closed: "\<And> a. a \<in> set assumptions \<Longrightarrow> closed a"
   assumes conclusions_closed: "\<And> c. c \<in> set conclusions \<Longrightarrow> closed c"
   assumes no_empty_conclusions: "\<forall>xs\<in>sset rules. consequent xs \<noteq> []"
 begin
-  definition ass_forms where "ass_forms = fset_from_list (map (subst undefined) (map (freshen undefined) assumptions))"
-  definition conc_forms where "conc_forms = fset_from_list (map (subst undefined) (map (freshen undefined) conclusions))"
+  definition ass_forms where "ass_forms = fset_from_list assumptions"
+  definition conc_forms where "conc_forms = fset_from_list  conclusions"
+
+  lemma mem_ass_forms[simp]: "a |\<in>| ass_forms \<longleftrightarrow> a \<in> set assumptions"
+    by (auto simp add: ass_forms_def)
+  
+  lemma mem_conc_forms[simp]: "a |\<in>| conc_forms \<longleftrightarrow> a \<in> set conclusions"
+    by (auto simp add: conc_forms_def)
+
+  lemma subst_freshen_assumptions[simp]:
+    assumes "pf \<in> set assumptions"
+    shows "subst s (freshen a pf) = pf "
+      using assms assumptions_closed 
+      by (simp add: closed_fv freshen_def rename_closed subst_closed)
+
+  lemma subst_freshen_conclusions[simp]:
+    assumes "pf \<in> set conclusions"
+    shows "subst s (freshen a pf) = pf "
+      using assms conclusions_closed 
+      by (simp add: closed_fv freshen_def rename_closed subst_closed)
 
   lemma subst_freshen_in_ass_formsI:
     assumes "pf \<in> set assumptions"
     shows "subst s (freshen a pf) |\<in>| ass_forms"
-      using assms ass_forms_def assumptions_closed closed_eq by fastforce
+      using assms by simp
 
   lemma subst_freshen_in_conc_formsI:
     assumes "pf \<in> set conclusions"
     shows "subst s (freshen a pf) |\<in>| conc_forms"
-      using assms conc_forms_def conclusions_closed closed_eq by fastforce
+      using assms by simp
 end
 
 end
